src/cddl/pulse/CDDL.Pulse.AST.Gen.fst
@@ -1,0 +1,352 @@
+module CDDL.Pulse.AST.Gen
+include CDDL.Spec.AST.Driver
+module U32 = FStar.UInt32
+
+let filter_char (c: FStar.Char.char) : Tot bool =
+  let code = FStar.Char.u32_of_char c in
+  (code `U32.gte` FStar.Char.u32_of_char 'A' &&
+    code `U32.lte` FStar.Char.u32_of_char 'Z') ||
+  (code `U32.gte` FStar.Char.u32_of_char 'a' &&
+    code `U32.lte` FStar.Char.u32_of_char 'z') ||
+  (code `U32.gte` FStar.Char.u32_of_char '0' &&
+    code `U32.lte` FStar.Char.u32_of_char '9') ||
+  code = FStar.Char.u32_of_char '_'
+
+let filter_name (name: string) = 
+  FStar.String.string_of_list (List.Tot.filter filter_char (FStar.String.list_of_string name))
+
+let mk_validator_name (name: string) : string =
+  "validate_" ^ filter_name name
+
+let mk_impltype_name (name: string) : string =
+  "impltype_" ^ filter_name name
+
+let mk_parsertype_name (name: string) : string =
+  "parsertype_" ^ filter_name name
+
+let mk_parser_name (name: string) : string =
+  "parse_" ^ filter_name name
+
+let krml = "\"krml\""
+
+let extend_ancillaries' env' ancillary_env source source' =
+"let _ : unit = _ by (FStar.Tactics.print (\"ancillary envs\"); FStar.Tactics.exact (`()))
+[@@noextract_to "^krml^"; sem_attr; bundle_attr] noextract
+let av"^env'^"_0 : Parse.ancillary_validate_env Det.cbor_det_match "^env'^".be_ast.e_sem_env =
+  Parse.ancillary_validate_env_extend av"^ancillary_env^" _
+[@@noextract_to "^krml^"; sem_attr; bundle_attr] noextract
+let a"^env'^"_0 : ancillary_bundle_env Det.cbor_det_match "^env'^".be_ast.e_sem_env =
+  ancillary_bundle_env_extend a"^ancillary_env^" _
+[@@noextract_to "^krml^"; sem_attr; bundle_attr] noextract
+let aa"^env'^"_0 : ancillary_array_bundle_env Det.cbor_det_array_iterator_match "^env'^".be_ast.e_sem_env =
+  ancillary_array_bundle_env_extend aa"^ancillary_env^" _
+let _ : unit = _ by (FStar.Tactics.print (\"source'\"); FStar.Tactics.exact (`()))
+[@@FStar.Tactics.postprocess_with (fun _ -> FStar.Tactics.norm [delta; zeta; iota; primops]; FStar.Tactics.trefl ()); noextract_to "^krml^"; base_attr] noextract
+let "^source'^" = List.Tot.tl "^source^"
+"
+
+let extend_ancillaries_for_typ env env' ancillary_index source source' =
+  extend_ancillaries' env' (env ^ "_" ^ string_of_int ancillary_index) source source'
+
+let extend_ancillaries_for_array_group env env' source source' =
+  extend_ancillaries' env' (env ^ "_0") source source'
+
+let call_ask_for_base wf ancillaries =
+  "Parse.ask_zero_copy_wf_type "^ancillaries^" "^wf
+
+let call_ask_for_aux candidate ancillaries =
+  "Parse.ask_zero_copy_ask_for_option "^ancillaries^" "^candidate
+
+let compute_ancillary_env env ancillary_index =
+  let env_ancillary_index = env ^ "_" ^ string_of_int ancillary_index in
+  "av"^env_ancillary_index^" a"^env_ancillary_index^" aa"^env_ancillary_index
+
+module P = CDDL.Pulse.AST.Parse
+
+noeq
+type ancillaries_t (se: sem_env) = {
+  validators: P.ancillary_validate_env_bool se.se_bound;
+  parsers: P.ancillary_parse_env_bool se;
+  array_parsers: P.ancillary_parse_array_group_env_bool se;
+}
+
+noeq
+type ancillaries_aux_t (se: sem_env) = {
+  anc: ancillaries_t se;
+  next_candidate_index: pos;
+  env_index: nat;
+  output: string;
+}
+
+let compute_wf_typ_ret
+  (env: sem_env)
+= result (nat & ((ancillaries_t env -> option (P.ask_for env)) & wf_ast_env))
+
+let compute_wf_typ_post
+  (env: wf_ast_env)
+  (res: compute_wf_typ_ret env.e_sem_env)
+: Tot prop
+= match res with
+  | ROutOfFuel -> False
+  | RFailure _ -> True
+  | RSuccess (_, (_, env')) -> ast_env_included env env'
+
+let rec compute_wf_typ
+  (env: wf_ast_env)
+  (name: string)
+  (t: typ)
+  (fuel: nat)
+: FStar.Tactics.Tac (res: compute_wf_typ_ret env.e_sem_env { compute_wf_typ_post env res })
+= if None? (env.e_sem_env.se_bound name)
+  then match mk_wf_typ' fuel env t with
+  | RFailure s -> RFailure s
+  | ROutOfFuel -> compute_wf_typ env name t (fuel + 1)
+  | RSuccess wt ->
+    let f (anc: ancillaries_t env.e_sem_env) : Tot (option (P.ask_for env.e_sem_env)) =
+      P.ask_zero_copy_wf_type anc.validators anc.parsers anc.array_parsers wt
+    in
+    RSuccess (fuel, (f, wf_ast_env_extend_typ_with_weak env name t wt))
+  else RFailure (name ^ " is already defined")
+
+let produce_validator env wf validator =
+"let _ : unit = _ by (FStar.Tactics.print (\"validator\"); FStar.Tactics.exact (`()))
+[@@FStar.Tactics.postprocess_for_extraction_with (fun _ -> FStar.Tactics.norm (nbe :: T.steps); FStar.Tactics.trefl ())]
+let "^validator^" = Impl.validate_typ Det.cbor_det_impl "^env^".be_v true _ "^wf
+
+let produce_parser env env_anc' wf validator parser bundle =
+produce_validator env wf validator^"
+let _ : unit = _ by (FStar.Tactics.print (\"bundle\"); FStar.Tactics.exact (`()))
+noextract [@@noextract_to "^krml^"; bundle_attr; bundle_get_impl_type_attr]
+let "^bundle^"' = impl_bundle_wf_type' Det.cbor_det_impl "^env^" av"^env_anc'^" a"^env_anc'^" aa"^env_anc'^" "^wf^" (_ by (T.trefl_or_norm ()))
+let _ : unit = _ by (FStar.Tactics.print (\"parser\"); FStar.Tactics.exact (`()))
+[@@FStar.Tactics.postprocess_for_extraction_with (fun _ -> FStar.Tactics.norm (nbe :: T.bundle_steps); FStar.Tactics.trefl ()); FStar.Tactics.postprocess_type]
+let "^parser^" = "^bundle^"'.b_parser
+let _ : unit = _ by (FStar.Tactics.print (\"bundle'\"); FStar.Tactics.exact (`()))
+inline_for_extraction noextract [@@noextract_to "^krml^"; bundle_attr; bundle_get_impl_type_attr]
+let "^bundle^" = { "^bundle^"' with b_parser = "^parser^" }
+let _ : unit = _ by (FStar.Tactics.print (\"env'\"); FStar.Tactics.exact (`()))"
+
+let rec compute_ancillaries_aux
+  (#se: sem_env)
+  (anc: ancillaries_aux_t se)
+  (current_candidate_index: nat)
+  (ask: option (P.ask_for se))
+: FStar.Tactics.Tac (ancillaries_aux_t se)
+= match P.ask_zero_copy_ask_for_option anc.anc.validators anc.anc.parsers anc.anc.array_parsers ask with
+  | None ->
+    begin match ask with
+    | None -> anc
+    | Some (P.AskForType t _ false) ->
+      { anc with
+        anc = {
+          anc.anc with
+          validators = (fun v -> if v = t then true else anc.anc.validators v);
+        };
+        env_index = anc.env_index + 1;
+      }
+    | Some (P.AskForType t t_wf true) ->
+      { anc with
+        anc = {
+          anc.anc with
+          parsers = (fun t' t_wf' -> if t = t' && t_wf = t_wf' then true else anc.anc.parsers t' t_wf');
+        };
+        env_index = anc.env_index + 1;
+      }
+    | Some (P.AskForArrayGroup t t_wf) ->
+      { anc with
+        anc = {
+          anc.anc with
+          array_parsers = (fun t' t_wf' -> if t = t' && t_wf = t_wf' then true else anc.anc.array_parsers t' t_wf');
+        };
+        env_index = anc.env_index + 1;
+      }
+    end
+  | ask' ->
+    let anc1 = {
+      anc with
+      next_candidate_index = anc.next_candidate_index + 1;
+    }
+    in
+    let anc2 = compute_ancillaries_aux anc1 anc.next_candidate_index ask' in
+    compute_ancillaries_aux anc2 current_candidate_index ask
+
+let rec compute_ancillaries
+  (#se: sem_env)
+  (init: ancillaries_t se -> option (P.ask_for se))
+  (anc: ancillaries_aux_t se)
+: FStar.Tactics.Tac (anc': ancillaries_aux_t se {
+    None? (init anc'.anc)
+  })
+= match init anc.anc with
+  | None -> anc
+  | ask ->
+    let anc1 = {
+      anc with
+      next_candidate_index = anc.next_candidate_index + 1;
+    }
+    in
+    let anc2 = compute_ancillaries_aux anc1 anc.next_candidate_index ask in
+    compute_ancillaries init anc2
+
+let extend_ancillaries_t
+  (#se: sem_env)
+  (anc: ancillaries_t se)
+  (se': sem_env { sem_env_included se se' })
+: Tot (ancillaries_t se')
+= let ne = se.se_bound in
+  {
+    validators = (fun t -> if typ_bounded ne t then anc.validators t else false);
+    parsers = (fun t t_wf -> if typ_bounded ne t && bounded_wf_typ ne _ t_wf then anc.parsers t t_wf else false);
+    array_parsers = (fun t t_wf -> if group_bounded ne t && bounded_wf_array_group ne _ t_wf then anc.array_parsers t t_wf else false);
+  }
+
+let produce_typ_defs_t : Type0
+= result (string & (wenv': wf_ast_env & ancillaries_t wenv'.e_sem_env))
+
+let produce_typ_defs_post
+  (wenv: wf_ast_env)
+  (res: produce_typ_defs_t)
+: Tot prop
+= match res with
+  | RFailure _ -> True
+  | ROutOfFuel -> False
+  | RSuccess (_, (| wenv', _ |)) -> ast_env_included wenv wenv'
+
+let produce_typ_defs
+  (index: nat)
+  (wenv: wf_ast_env)
+  (anc: ancillaries_t wenv.e_sem_env)
+  (name: string)
+  (t: typ)
+: FStar.Tactics.Tac (res: produce_typ_defs_t { produce_typ_defs_post wenv res })
+= match compute_wf_typ wenv name t 0 with
+  | RFailure s -> RFailure s
+  | RSuccess (fuel, (f, wenv')) ->
+  let i = string_of_int index in
+  let j = string_of_int (index + 1) in
+  let validator = mk_validator_name name in
+  let impltype = mk_impltype_name name in
+  let parsertype = mk_parsertype_name name in
+  let parser = mk_parser_name name in
+  let wf = "wf" ^ j in
+  let env = "env" ^ i in
+  let env' = "env" ^ j in
+  let ask = "ask" ^ j in
+  let source = "sorted_source" ^ i in
+  let source' = "sorted_source" ^ j in
+  let bundle = "b" ^ j in
+  let fuel = string_of_int fuel in
+  let anc1 = compute_ancillaries f {
+    anc = anc;
+    env_index = 0;
+    next_candidate_index = 1;
+    output = "";
+  }
+  in
+  let env_anc' = env ^ "_" ^ string_of_int anc1.env_index in
+  let anc' : ancillaries_t wenv'.e_sem_env = extend_ancillaries_t anc1.anc wenv'.e_sem_env in
+  let msg =
+"
+let _ : unit = _ by (FStar.Tactics.print (\"owf'\"); FStar.Tactics.exact (`()))
+[@@noextract_to "^krml^"] noextract
+let o"^wf^"' = compute_wf_typ' "^env^".be_ast (T.pull_name "^source^") (_ by (T.trefl_or_norm ())) (T.pull_type "^source^") "^fuel^"
+let _ : unit = _ by (FStar.Tactics.print (\"owf\"); FStar.Tactics.exact (`()))
+[@@FStar.Tactics.postprocess_with (fun _ -> FStar.Tactics.norm [delta; zeta; iota; primops]; FStar.Tactics.trefl ()); noextract_to "^krml^"] noextract
+let o"^wf^" = o"^wf^"'
+let o"^wf^"_eq : squash (o"^wf^" == o"^wf^"') = _ by (T.trefl_or_norm ())
+let _ : unit = _ by (FStar.Tactics.print (\"wf'\"); FStar.Tactics.exact (`()))
+[@@noextract_to "^krml^"] noextract
+let "^wf^"' = extract_computed_wf_typ' "^env^".be_ast (T.pull_name "^source^") (T.pull_type "^source^") "^fuel^" o"^wf^" (_ by (T.trefl_or_norm ()))
+let _ : unit = _ by (FStar.Tactics.print (\"wf\"); FStar.Tactics.exact (`()))
+[@@FStar.Tactics.postprocess_with (fun _ -> FStar.Tactics.norm [delta; zeta; iota; primops]; FStar.Tactics.trefl ()); noextract_to "^krml^"; base_attr] noextract
+let "^wf^" = "^wf^"'
+let _ : squash ("^wf^" == "^wf^"') = _ by (T.trefl_or_norm ())
+"^anc1.output^produce_parser env env_anc' wf validator parser bundle ^"
+[@@noextract_to "^krml^"; sem_attr; bundle_attr] noextract
+let "^env'^" =
+  bundle_env_extend_typ_with_weak "^env^" (T.pull_name "^source^") (T.pull_type "^source^") "^wf^" "^validator^" "^bundle^"
+" ^ extend_ancillaries_for_typ env env' anc1.env_index source source'
+in
+  RSuccess (msg, (| wenv', anc' |))
+
+let produce_group_defs
+  (wenv: wf_ast_env)
+  (anc: ancillaries_t wenv.e_sem_env)
+  (name: string)
+  (g: group)
+  (index: nat)
+: Tot (res: produce_typ_defs_t { produce_typ_defs_post wenv res })
+= if Some? (wenv.e_sem_env.se_bound name)
+  then RFailure (name ^ " already defined")
+  else if not (group_bounded wenv.e_sem_env.se_bound g)
+  then RFailure (name ^ " : group not bounded. We do not support recursive CDDL groups yet")
+  else
+  let wenv' = wf_ast_env_extend_group wenv name g () () in
+  let i = string_of_int index in
+  let j = string_of_int (index + 1) in
+  let env = "env" ^ i in
+  let env' = "env" ^ j in
+  let source = "sorted_source" ^ i in
+  let source' = "sorted_source" ^ j in
+  let msg =
+(
+"
+let _ : unit = _ by (FStar.Tactics.print (\"env'\"); FStar.Tactics.exact (`()))
+[@@noextract_to "^krml^"; sem_attr; bundle_attr] noextract
+let "^env'^" =
+  bundle_env_extend_group "^env^" (T.pull_name "^source^") (T.pull_group "^source^") (_ by (T.trefl_or_norm ())) (_ by (T.trefl_or_norm ()))
+" ^ extend_ancillaries_for_array_group env env' source source'
+)
+  in
+  RSuccess (msg, (| wenv', extend_ancillaries_t anc _ |))
+
+let rec produce_defs'
+  (index: nat)
+  (accu: string)
+  (env: wf_ast_env)
+  (anc: ancillaries_t env.e_sem_env)
+  (l: list (string & decl))
+: FStar.Tactics.Tac (res: result string { ~ (ROutOfFuel? res) })
+= match l with
+  | [] -> RSuccess accu
+  | (name, def) :: q ->
+    let accu = accu ^
+"
+let _ : unit = _ by (FStar.Tactics.print (\"" ^ string_of_int (List.Tot.length l) ^ " defs remaining. Producing definitions for "^name^"\"); FStar.Tactics.exact (`()))
+"
+    in
+    begin match def with
+    | DType t ->
+      begin match produce_typ_defs index env anc name t with
+      | RSuccess (msg, (| env', anc' |)) ->
+        produce_defs' (index + 1) (accu ^ msg) env' anc' q
+      | RFailure s -> RFailure s
+      end
+    | DGroup g ->
+      begin match produce_group_defs env anc name g index with
+      | RFailure s -> RFailure s
+      | RSuccess (msg, (| env', anc' |)) ->
+        produce_defs' (index + 1) (accu ^ msg) env' anc' q
+      end
+    end
+
+let empty_ancillaries : ancillaries_t empty_sem_env = {
+  validators = (fun _ -> false);
+  parsers = (fun _ _ -> false);
+  array_parsers = (fun _ _ -> false);
+}
+
+let produce_defs
+  (l: list (string & decl))
+: FStar.Tactics.Tac unit
+= let accu = "
+*)
+" in
+  match produce_defs' 0 accu empty_wf_ast_env empty_ancillaries l with
+  | RFailure s -> FStar.Tactics.fail s
+  | RSuccess msg -> let msg = msg ^ "
+(*
+"
+    in
+    FStar.Tactics.print msg;
+    FStar.Tactics.exact (`())
